Notations and fancier pure term checker\n\nAdded some notations to save time typing all the names, also rewrote the pure term checking so that it matches more with the papers version, wrote some lemmas for it too.

src/semantic_rules.v
@@ -5,49 +5,6 @@ From stdpp Require Export strings.
 From stdpp Require Import stringmap.
 
 
-(* --- Pure term validation ------------------------------------------------------ *)
-
-(*
-Pure terms are:
-- variables whose essential type is a base type
-- constants with simple type (τb1 → τb2 → ... → τbn)
-- application of pure terms to pure terms
- *)
-
-Fixpoint is_simple_type (type : i_ty) : bool :=
-  match type with
-  | TBase _ => true
-  | TArr t1 t2 => is_simple_type t1 && is_simple_type t2
-  | TProd t1 t2 => is_simple_type t1 && is_simple_type t2
-  | _ => false
-  end.
-
-Definition essential_type_is_base_type (type : i_ty) : bool :=
-  match type with
-  | TBase _ => true
-  | TSet _ _ _ => true
-  | _ => false
-  end.
-
-Fixpoint is_pure_term (term : i_expr) (var_con : var_context) (const_con : const_context) : bool :=
-  match term with
-  | EConst con_name => match (const_ctx_lookup const_con con_name) with
-    | Some type => is_simple_type type
-    | _ => false
-    end
-  | EVar var_name => match (var_ctx_lookup var_con var_name) with
-    | Some type => essential_type_is_base_type type
-    | _ => false
-    end
-  | EApp exp1 exp2 => is_pure_term exp1 var_con const_con && is_pure_term exp2 var_con const_con
-  | _ => false
-  end.
-
-(* Some testing just in case *)
-Compute is_pure_term (EApp (EConst "f") (EVar "a")) [] [].
-Compute is_pure_term (EApp (EConst "f") (EVar "a")) [("a"%string , TSet "x" BBool (EBool false))] [].
-Compute is_pure_term (EApp (EConst "f") (EVar "a")) [("a"%string , TSet "x" BBool (EConst "b"))] [("f"%string , TArr (TBase BBool) (TBase BBool))].
-
 (* --- Selfification rule ------------------------------------------------------ *)
 
 Fixpoint exp_vars (term : i_expr) : list string :=
@@ -94,3 +51,110 @@ Fixpoint self (type : i_ty) (term : i_expr) : i_ty :=
 
 Compute self (TBase BNat) (EVar ("x"%string)).
 Compute self (TArr (TBase BNat) (TArr (TBase BNat) (TBase BNat))) (EVar ("+"%string)).
+
+
+(* --- Pure term validation ------------------------------------------------------ *)
+
+(*
+Pure terms are:
+- variables whose essential type is a base type
+- constants with simple type (τb1 → τb2 → ... → τbn)
+- application of pure terms to pure terms
+ *)
+
+Fixpoint is_simple_type (type : i_ty) : bool :=
+  match type with
+  | TBase _ => true
+  | TArr t1 t2 => is_simple_type t1 && is_simple_type t2
+  | TProd t1 t2 => is_simple_type t1 && is_simple_type t2
+  | _ => false
+  end.
+
+Definition essential_type_is_base_type (type : i_ty) : bool :=
+  match type with
+  | TBase _ => true
+  | TSet _ _ _ => true
+  | _ => false
+  end.
+Notation "β[ t ]" := (essential_type_is_base_type t) (at level 10).
+
+
+(* Fixpoint is_pure_term (term : i_expr) (var_con : var_context) (const_con : const_context) : bool :=
+  match term with
+  | EConst con_name => match (const_ctx_lookup const_con con_name) with
+    | Some type => is_simple_type type
+    | _ => false
+    end
+  | EVar var_name => match (var_ctx_lookup var_con var_name) with
+    | Some type => essential_type_is_base_type type
+    | _ => false
+    end
+  | EApp exp1 exp2 => is_pure_term exp1 var_con const_con && is_pure_term exp2 var_con const_con
+  | _ => false
+  end.
+
+(* Some testing just in case *)
+Compute is_pure_term (EApp (EConst "f") (EVar "a")) [] [].
+Compute is_pure_term (EApp (EConst "f") (EVar "a")) [("a"%string , TSet "x" BBool (EBool false))] [].
+Compute is_pure_term (EApp (EConst "f") (EVar "a")) [("a"%string , TSet "x" BBool (EConst "b"))] [("f"%string , TArr (TBase BBool) (TBase BBool))]. *)
+
+
+
+(* Fancier way *)
+
+Inductive has_type_pure
+  (var_con : var_context)
+  (const_con : const_context)
+  : i_expr -> i_ty -> Prop :=
+  | PVar :
+    forall x τb,
+      Γ[ x ] var_con = Some τb ->
+      β[ τb ] ->
+      has_type_pure var_con const_con (EVar x) τb
+  | PNat :
+    forall n,
+    has_type_pure var_con const_con (ENat n) (TBase BNat)
+  | PBool :
+    forall b,
+    has_type_pure var_con const_con (EBool b) (TBase BBool)
+  | PString :
+    forall s,
+    has_type_pure var_con const_con (EString s) (TBase BString)
+  | PUnit :
+    forall u,
+    has_type_pure var_con const_con (EUnit u) (TBase BUnit)
+  | PConst :
+    forall c τ,
+      Φ[ c ] const_con = Some τ ->
+      is_simple_type τ ->
+      has_type_pure var_con const_con (EConst c) τ
+  | PApp :
+    forall e₁ e₂ τ₁ τ₂,
+      β[ τ₁ ] ->
+      has_type_pure var_con const_con e₁ (TArr τ₁ τ₂) ->
+      has_type_pure var_con const_con e₂ τ₁ ->
+      has_type_pure var_con const_con (EApp e₁ e₂) τ₂.
+
+Lemma pure_plus_app_nat :
+  has_type_pure [( "n" , TBase BNat)] [( "+" , TArr (TBase BNat) (TArr (TBase BNat) (TBase BNat)))] (EApp (EConst "+"%string) (ENat 1)) (TArr (TBase BNat) (TBase BNat)).
+  Proof.
+  apply (PApp _ _ _ _ (TBase BNat) _).
+  - simpl. reflexivity.
+  - apply PConst.
+    + simpl. reflexivity.
+    + simpl. reflexivity.
+  - apply PNat.
+  Qed.
+
+Lemma pure_plus_app_var :
+  has_type_pure [( "n" , TBase BNat)] [( "+" , TArr (TBase BNat) (TArr (TBase BNat) (TBase BNat)))] (EApp (EConst "+"%string) (EVar "n")) (TArr (TBase BNat) (TBase BNat)).
+  Proof.
+  apply (PApp _ _ _ _ (TBase BNat) _).
+  - simpl. reflexivity.
+  - apply PConst.
+    + simpl. reflexivity.
+    + simpl. reflexivity.
+  - apply PVar.
+    + simpl. reflexivity.
+    + simpl. reflexivity.
+  Qed.
